some cleanup

src/tls/HSL.Receive.fst
@@ -74,24 +74,6 @@ let create r =
   let inc_st = B.malloc r (G.hide (Seq.empty, F_none)) 1ul in
   { rgn = r; inc_st = inc_st }
 
-(***** TODO: these errors should move somewhere
-       so that clients can match on them *****)
-
-let parsing_error : TLSError.error = {
-  Parsers.Alert.level = Parsers.AlertLevel.Fatal;
-  Parsers.Alert.description = Parsers.AlertDescription.Unexpected_message
-}, ""
-
-let unexpected_flight_error : TLSError.error = {
-  Parsers.Alert.level = Parsers.AlertLevel.Fatal;
-  Parsers.Alert.description = Parsers.AlertDescription.Unexpected_message
-}, ""
-
-let bytes_remain_error : TLSError.error = {
-  Parsers.Alert.level = Parsers.AlertLevel.Fatal;
-  Parsers.Alert.description = Parsers.AlertDescription.Unexpected_message
-}, ""
-
 
 /// Main workhorse of parsing messages
 ///
@@ -117,30 +99,30 @@ let parse_common
     forall (m:a1).
       (tag_fn m == tag) <==> cl.LP.clens_cond m})
   (acc:LP.accessor gacc)
-  : b:R.const_slice -> from:uint_32 ->
+  : b:R.const_slice -> f_begin:uint_32 ->
     Stack (TLSError.result (option (R.repr_p a1 b p1 & uint_32)))
     (requires fun h ->
       R.live h b /\
-      from <= b.R.len)
+      f_begin <= b.R.len)
     (ensures fun h0 r h1 ->
       B.modifies B.loc_none h0 h1 /\
       (match r with
        | E.Error _ -> True
        | E.Correct None -> True
        | E.Correct (Some (repr, pos)) ->  //on a successful parse it returns a valid repr with lens condition
-         repr.R.start_pos == from /\
+         repr.R.start_pos == f_begin /\
          repr.R.end_pos == pos /\
          R.valid repr h1 /\
          cl.LP.clens_cond (R.value repr)))
          
-  = fun b from ->
+  = fun b f_begin ->
     let lp_b = R.to_slice b in
-    let pos = validator lp_b from in  //validator gives us the valid postcondition
+    let pos = validator lp_b f_begin in  //validator gives us the valid postcondition
 
     if pos <= LP.validator_max_length then begin
-      let parsed_tag = HSMType.handshakeType_reader lp_b from in
+      let parsed_tag = HSMType.handshakeType_reader lp_b f_begin in
       if parsed_tag = tag then  //and this dynamic check gives us the lens postcondition
-        let r = R.mk_from_const_slice b from pos p1 in
+        let r = R.mk_from_const_slice b f_begin pos p1 in
         E.Correct (Some (r, pos))
       else E.Error unexpected_flight_error
     end
@@ -170,12 +152,12 @@ private let err_or_insufficient_data
   (#a:Type) (#t:Type)
   (parse_result:TLSError.result (option a))
   (in_progress:in_progress_flt_t)
-  (st:hsl_state) (b:R.const_slice) (from to:uint_32)
+  (st:hsl_state) (b:R.const_slice) (f_begin f_end:uint_32)
   : Stack (TLSError.result (option t))
     (requires fun h ->
       B.live h st.inc_st /\ R.live h b /\
       B.loc_disjoint (footprint st) (R.loc b) /\
-      from <= to /\ to <= b.R.len /\
+      f_begin <= f_end /\ f_end <= b.R.len /\
       (E.Error? parse_result \/ parse_result == E.Correct None))
     (ensures  fun h0 r h1 ->
       B.modifies (footprint st) h0 h1 /\
@@ -184,24 +166,33 @@ private let err_or_insufficient_data
        | E.Correct None ->
          r == E.Correct None /\
          parsed_bytes st h1 ==
-           Seq.slice (R.as_seq h0 b) (v from) (v to) /\
+           Seq.slice (R.as_seq h0 b) (v f_begin) (v f_end) /\
          in_progress_flt st h1 == in_progress))
   = match parse_result with
     | E.Error e -> E.Error e
     | E.Correct None ->
       let inc_st =
         let h = ST.get () in
-        let parsed_bytes = LP.bytes_of_slice_from_to h (R.to_slice b) from to in
+        let parsed_bytes = LP.bytes_of_slice_from_to h (R.to_slice b) f_begin f_end in
         G.hide (parsed_bytes, in_progress)
       in
       B.upd st.inc_st 0ul inc_st;
       E.Correct None
 
+/// Helper function to check that the end index matches with pos
+///   and then either return an error or the flight flt
+
+inline_for_extraction noextract
+let check_end_index_and_return (#a:Type) (st:hsl_state) (pos f_end:uint_32) (flt:a) =
+  if pos <> f_end then E.Error bytes_remain_error
+  else begin
+    reset_incremental_state st;
+    E.Correct (Some flt)
+  end
+
 
 (*** ClientHello and ServerHello flights ***)
 
-
-/// The flights parsing code is straightforward if..then..else using the parsing functions above
 
 inline_for_extraction noextract
 let parse_hsm_ch
@@ -219,33 +210,25 @@ let parse_hsm_sh
       HSMType.Server_hello
       HSM.handshake_accessor_server_hello
 
-let receive_s_Idle st b from to =
+let receive_s_Idle st b f_begin f_end =
   let flt = F_s_Idle in
 
-  let r = parse_hsm_ch b from in
+  let r = parse_hsm_ch b f_begin in
   match r with
   | E.Error _ | E.Correct None ->
-    err_or_insufficient_data r flt st b from to
+    err_or_insufficient_data r flt st b f_begin f_end
   | E.Correct (Some (ch_repr, pos)) ->
-    if pos <> to then E.Error bytes_remain_error
-    else begin
-      reset_incremental_state st;
-      E.Correct (Some ({ ch_msg = ch_repr }))
-    end
+    check_end_index_and_return st pos f_end ({ ch_msg = ch_repr })
 
-let receive_c_wait_ServerHello st b from to =
+let receive_c_wait_ServerHello st b f_begin f_end =
   let flt = F_c_wait_ServerHello in
 
-  let r = parse_hsm_sh b from in
+  let r = parse_hsm_sh b f_begin in
   match r with
   | E.Error _ | E.Correct None ->
-    err_or_insufficient_data r flt st b from to
+    err_or_insufficient_data r flt st b f_begin f_end
   | E.Correct (Some (sh_repr, pos)) ->
-    if pos <> to then E.Error bytes_remain_error
-    else begin
-      reset_incremental_state st;
-      E.Correct (Some ({ sh_msg = sh_repr }))
-    end
+    check_end_index_and_return st pos f_end ({sh_msg = sh_repr})
 
 
 (*** 1.3 flights ***)
@@ -309,24 +292,27 @@ let parse_hsm13_nst
       HSMType.New_session_ticket
       HSM13.handshake13_accessor_new_session_ticket
 
+
+/// Helper function to parse c13 and cv13 that appear together in a flight
+
 private let parse_hsm13_c_cv
-  (b:R.const_slice) (from:uint_32)
+  (b:R.const_slice) (f_begin:uint_32)
   : Stack (TLSError.result (option (HSM13R.c13_repr b & HSM13R.cv13_repr b & uint_32)))
     (requires fun h ->
       R.live h b /\
-      from <= b.R.len)
+      f_begin <= b.R.len)
     (ensures fun h0 r h1 ->
       B.modifies B.loc_none h0 h1 /\
       (match r with
        | E.Error _ -> True
        | E.Correct None -> True
        | E.Correct (Some (c13, cv13, pos)) ->
-         c13.R.start_pos == from /\
+         c13.R.start_pos == f_begin /\
          c13.R.end_pos == cv13.R.start_pos /\
          cv13.R.end_pos == pos /\
          R.valid c13 h1 /\
          R.valid cv13 h1))
-  = let r = parse_hsm13_c b from in
+  = let r = parse_hsm13_c b f_begin in
     match r with
     | E.Error e -> E.Error e
     | E.Correct None -> E.Correct None
@@ -339,18 +325,18 @@ private let parse_hsm13_c_cv
         E.Correct (Some (c_repr, cv_repr, cv_end))
 
 #set-options "--z3rlimit 50"
-let receive_c13_wait_Finished1 st b from to =
+let receive_c13_wait_Finished1 st b f_begin f_end =
   let flt = F_c13_wait_Finished1 in
 
-  let r = parse_hsm13_ee b from in
+  let r = parse_hsm13_ee b f_begin in
   match r with
   | E.Error _ | E.Correct None ->
-    err_or_insufficient_data r flt st b from to
+    err_or_insufficient_data r flt st b f_begin f_end
   | E.Correct (Some (ee_repr, ee_end)) ->
     let r = parse_hsm13_cr b ee_end in
     match r with
     | E.Correct None ->
-      err_or_insufficient_data r flt st b from to
+      err_or_insufficient_data r flt st b f_begin f_end
     | _ ->
      let cr_repr, c_cv_begin =
        match r with
@@ -361,7 +347,7 @@ let receive_c13_wait_Finished1 st b from to =
      let r = parse_hsm13_c_cv b c_cv_begin in
      match r with
      | E.Correct None ->
-       err_or_insufficient_data r flt st b from to
+       err_or_insufficient_data r flt st b f_begin f_end
      | _ ->
        let c_cv_repr, fin_begin =
          match r with
@@ -372,78 +358,60 @@ let receive_c13_wait_Finished1 st b from to =
        let r = parse_hsm13_fin b fin_begin in
        match r with
        | E.Error _ | E.Correct None ->
-         err_or_insufficient_data r flt st b from to
+         err_or_insufficient_data r flt st b f_begin f_end
        | E.Correct (Some (fin_repr, fin_end)) ->
-         if fin_end <> to then E.Error bytes_remain_error
-         else begin
-           reset_incremental_state st;
-           E.Correct (Some ({
-             ee_msg = ee_repr;
-             cr_msg = cr_repr;
-             c_cv_msg = c_cv_repr;
-             fin_msg = fin_repr
-           }))
-         end
+         check_end_index_and_return st fin_end f_end ({
+           ee_msg = ee_repr;
+           cr_msg = cr_repr;
+           c_cv_msg = c_cv_repr;
+           fin_msg = fin_repr
+         })
 
-let receive_s13_wait_Finished2 st b from to =
+let receive_s13_wait_Finished2 st b f_begin f_end =
   let flt = F_s13_wait_Finished2 in
 
-  let r = parse_hsm13_c_cv b from in
+  let r = parse_hsm13_c_cv b f_begin in
   match r with
-  | E.Correct None -> err_or_insufficient_data r flt st b from to
+  | E.Correct None -> err_or_insufficient_data r flt st b f_begin f_end
   | _ ->
     let c_cv_repr, fin_begin =
       match r with
-      | E.Error _ -> None, from
+      | E.Error _ -> None, f_begin
       | E.Correct (Some (c_repr, cv_repr, c_cv_end)) ->
         Some (c_repr, cv_repr), c_cv_end
     in
     let r = parse_hsm13_fin b fin_begin in
     match r with
-    | E.Error _ | E.Correct None -> err_or_insufficient_data r flt st b from to
+    | E.Error _ | E.Correct None -> err_or_insufficient_data r flt st b f_begin f_end
     | E.Correct (Some (fin_repr, fin_end)) ->
-      if fin_end <> to then E.Error bytes_remain_error
-      else begin
-        reset_incremental_state st;
-        E.Correct (Some ({
-          c_cv_msg = c_cv_repr;
-          fin_msg = fin_repr
-        }))
-      end
+      check_end_index_and_return st fin_end f_end ({
+        c_cv_msg = c_cv_repr;
+        fin_msg = fin_repr
+      })
 
-let receive_s13_wait_EOED st b from to =
+let receive_s13_wait_EOED st b f_begin f_end =
   let flt = F_s13_wait_EOED in
 
-  let r = parse_hsm13_eoed b from in
+  let r = parse_hsm13_eoed b f_begin in
   match r with
   | E.Error _ | E.Correct None ->
-    err_or_insufficient_data r flt st b from to
+    err_or_insufficient_data r flt st b f_begin f_end
   | E.Correct (Some (eoed_repr, pos)) ->
-    if pos <> to then E.Error bytes_remain_error
-    else begin
-      reset_incremental_state st;
-      E.Correct (Some ({ eoed_msg = eoed_repr }))
-    end
+    check_end_index_and_return st pos f_end ({ eoed_msg = eoed_repr })
 
-let receive_c13_Complete st b from to =
+let receive_c13_Complete st b f_begin f_end =
   let flt = F_c13_Complete in
 
-  let r = parse_hsm13_nst b from in
+  let r = parse_hsm13_nst b f_begin in
   match r with
   | E.Error _ | E.Correct None ->
-    err_or_insufficient_data r flt st b from to
+    err_or_insufficient_data r flt st b f_begin f_end
   | E.Correct (Some (nst_repr, pos)) ->
-    if pos <> to then E.Error bytes_remain_error
-    else begin
-      reset_incremental_state st;
-      E.Correct (Some ({ nst_msg = nst_repr }))
-    end
+    check_end_index_and_return st pos f_end ({ nst_msg = nst_repr })
 
 
 (*** 1.2 flights ***)
 
-
-/// Specialize the parse_common function for Handshake12 messages
 
 inline_for_extraction noextract
 let parse_hsm12_c
@@ -502,20 +470,20 @@ let parse_hsm12_cke
       HSM12.handshake12_accessor_client_key_exchange
 
 
-let receive_c12_wait_ServerHelloDone st b from to =
+let receive_c12_wait_ServerHelloDone st b f_begin f_end =
   let flt = F_c12_wait_ServerHelloDone in
 
-  let r = parse_hsm12_c b from in
+  let r = parse_hsm12_c b f_begin in
   match r with
-  | E.Error _ | E.Correct None -> err_or_insufficient_data r flt st b from to
+  | E.Error _ | E.Correct None -> err_or_insufficient_data r flt st b f_begin f_end
   | E.Correct (Some (c_repr, c_end)) ->
     let r = parse_hsm12_ske b c_end in
     match r with
-    | E.Error _ | E.Correct None -> err_or_insufficient_data r flt st b from to
+    | E.Error _ | E.Correct None -> err_or_insufficient_data r flt st b f_begin f_end
     | E.Correct (Some (ske_repr, ske_end)) ->
       let r = parse_hsm12_cr b ske_end in
       match r with
-      | E.Correct None -> err_or_insufficient_data r flt st b from to
+      | E.Correct None -> err_or_insufficient_data r flt st b f_begin f_end
       | _ ->
         let cr_repr, shd_begin =
           match r with
@@ -525,56 +493,41 @@ let receive_c12_wait_ServerHelloDone st b from to =
         let r = parse_hsm12_shd b shd_begin in
         match r with
         | E.Error _ | E.Correct None ->
-          err_or_insufficient_data r flt st b from to
+          err_or_insufficient_data r flt st b f_begin f_end
         | E.Correct (Some (shd_repr, pos)) ->
-          if pos <> to then E.Error bytes_remain_error
-          else begin
-            reset_incremental_state st;
-            E.Correct (Some ({
-              c_msg = c_repr;
-              ske_msg = ske_repr;
-              cr_msg = cr_repr;
-              shd_msg = shd_repr }))
-          end
+          check_end_index_and_return st pos f_end ({
+            c_msg = c_repr;
+            ske_msg = ske_repr;
+            cr_msg = cr_repr;
+            shd_msg = shd_repr
+          })
 
-let receive_cs12_wait_Finished st b from to =
+let receive_cs12_wait_Finished st b f_begin f_end =
   let flt = F_cs12_wait_Finished in
 
-  let r = parse_hsm12_fin b from in
+  let r = parse_hsm12_fin b f_begin in
   match r with
   | E.Error _ | E.Correct None ->
-    err_or_insufficient_data r flt st b from to
+    err_or_insufficient_data r flt st b f_begin f_end
   | E.Correct (Some (fin_repr, pos)) ->
-    if pos <> to then E.Error bytes_remain_error
-    else begin
-      reset_incremental_state st;
-      E.Correct (Some ({ fin_msg = fin_repr }))
-    end
+    check_end_index_and_return st pos f_end ({ fin_msg = fin_repr })
 
-let receive_c12_wait_NST st b from to =
+let receive_c12_wait_NST st b f_begin f_end =
   let flt = F_c12_wait_NST in
 
-  let r = parse_hsm12_nst b from in
+  let r = parse_hsm12_nst b f_begin in
   match r with
   | E.Error _ | E.Correct None ->
-    err_or_insufficient_data r flt st b from to
+    err_or_insufficient_data r flt st b f_begin f_end
   | E.Correct (Some (nst_repr, pos)) ->
-    if pos <> to then E.Error bytes_remain_error
-    else begin
-      reset_incremental_state st;
-      E.Correct (Some ({ nst_msg = nst_repr }))
-    end
+    check_end_index_and_return st pos f_end ({ nst_msg = nst_repr })
 
-let receive_s12_wait_CCS1 st b from to =
+let receive_s12_wait_CCS1 st b f_begin f_end =
   let flt = F_s12_wait_CCS1 in
 
-  let r = parse_hsm12_cke b from in
+  let r = parse_hsm12_cke b f_begin in
   match r with
   | E.Error _ | E.Correct None ->
-    err_or_insufficient_data r flt st b from to
+    err_or_insufficient_data r flt st b f_begin f_end
   | E.Correct (Some (cke_repr, pos)) ->
-    if pos <> to then E.Error bytes_remain_error
-    else begin
-      reset_incremental_state st;
-      E.Correct (Some ({ cke_msg = cke_repr }))
-    end
+    check_end_index_and_return st pos f_end ({ cke_msg = cke_repr })
